# baseURI: http://linked.data.gov.au/def/geofabric
# imports: http://www.opengis.net/ont/geosparql#

@prefix : <http://linked.data.gov.au/def/geofabric#> .
@prefix dc: <http://purl.org/dc/elements/1.1/> .
@prefix dct: <http://purl.org/dc/terms/> .
@prefix geo: <http://www.opengis.net/ont/geosparql#> .
@prefix hyf: <https://www.opengis.net/def/appschema/hy_features/hyf/> .
@prefix owl: <http://www.w3.org/2002/07/owl#> .
@prefix rdf: <http://www.w3.org/1999/02/22-rdf-syntax-ns#> .
@prefix rdfs: <http://www.w3.org/2000/01/rdf-schema#> .
@prefix sdo: <https://schema.org/> .
@prefix xml: <http://www.w3.org/XML/1998/namespace> .
@prefix xsd: <http://www.w3.org/2001/XMLSchema#> .

<http://linked.data.gov.au/def/geofabric>
  a owl:Ontology ;
  dct:contributor <https://orcid.org/0000-0002-3884-3420> ;
  dct:created "2019-06-07"^^xsd:date ;
  dct:creator [
      sdo:identifier <http://orcid.org/0000-0002-8742-7730> ;
      sdo:name "Nicholas J. Car" ;
    ] ;
  dct:modified "2019-07-29"^^xsd:date ;
  dct:publisher [
      sdo:identifier <http://catalogue.linked.data.gov.au/org/csiro> ;
      sdo:name "CSIRO" ;
    ] ;
  dct:source <http://www.bom.gov.au/water/geofabric/documents/v3_0/ahgf_productguide_V3_0_release.pdf> ;
  rdfs:comment """A bare-bones ontology for the Australian Hydrological Geospatial Fabric.

This small ontology characterises major parts of the [Australian Hydrological Geospatial Fabric](http://www.bom.gov.au/water/geofabric/) for their delivery as [Linked Data](https://www.w3.org/wiki/LinkedData) via the [Geofabric LDAPI](http://linked.data.gov.au/dataset/geofabric).

This ontology accords with the [Loc-I Project](http://locationindex.org)'s requirements for the delivery of spatial [Semantic Web](https://www.w3.org/standards/semanticweb/) objects."""@en ;
  rdfs:label "Geofabric Ontology"@en ;
  rdfs:seeAlso <http://www.bom.gov.au/water/geofabric/documents/v2_1/AHGF_GDB_ProductRelationships_V2_1_release.pdf> ;
  rdfs:seeAlso "http://github.com/CSIRO-enviro-informatics/geofabric-ont/"@en ;
  owl:imports geo: ;
  owl:versionIRI <http://linked.data.gov.au/def/geofabric/1.0> ;
  owl:versionInfo "Beta version"@en ;
  owl:versionInfo "Version 1.0 only characterises 3 types of Feature - Contracted Catchment, River Region & Drianage Division - and requires that each CC be within a RR and that an RR be within a DD."@en ;
.
:ContractedCatchment
  a owl:Class ;
  dc:description """All contracted catchment features of type ContractedArea are aggregations of the
AHGFCatchment units that participate in a relationship of common geographic extent based
upon the location of a contracted node from both Geofabric Surface Cartography and
Geofabric Surface Network or a data sink as defined within the DEM-1S. Levels of confidence
for contracted nodes are further described in the following section of the Geofabric Product
Guide.

Each ContractedArea is assigned with the contracted node identifier (ConNodeID) and the
confidence level (ConLevel) of the contracted node to which they drain. The ContractedArea
features are the drainage areas of a combination of Levels 1 and 2 contracted nodes. These
drainage areas also incorporate catchment areas where there is no discernable flow (at
1:250,000 scale) in the form of stream flow segment features. The allocation of no flow areas
to contracted catchments is performed based on the most likely destination of water falling in
these areas in flood type conditions. 

Contracted catchment hierarchy

In previous versions of the Geofabric, the set of contracted catchment features provided a
collection of drainage areas for a set of persistent contracted nodes. In V2.1 these areas have
been further processed to aggregate these features into a contracted catchment hierarchy.
This hierarchy of contracted catchments includes only those catchments for key contracted
nodes taken from a full set of contractible river confluences, sinks, monitoring points and the
inflow and outflow points of water storages. These key contracted nodes form a stable,
logical, dendritic hierarchy of catchments that can be reliably reproduced when moving to
higher resolution or larger scaled data. The contracted catchment hierarchy provides a
reliable and stable set of catchments that, among other things, can be mapped to a number
of types of water reporting areas (depending on the use case) as exemplified by the stable
reporting regions given in Hydrology Reporting Regions.""" ;
  dc:source "Section 5.4.3 Page 40 in the Australian Hydrological Geospatial Fabric (Geofabric) v3.0 Product Guide"@en ;
  rdfs:comment """The Geofabric's Hydrology Reporting Catchments product's AHGF Contracted Catchment object.

Contracted Catchments are always within River Revions."""@en ;
  rdfs:label "Contracted Catchment" ;
  rdfs:subClassOf geo:Feature ;
  rdfs:subClassOf hyf:HY_Catchment ;
  rdfs:subClassOf [
      a owl:Restriction ;
      owl:onClass :RiverRegion ;
      owl:onProperty geo:sfWithin ;
      owl:qualifiedCardinality "1"^^xsd:nonNegativeInteger ;
    ] ;
.
:DrainageDivision
  a owl:Class ;
  dc:description """The AWRA Drainage Division is defined for the purpose of providing a stable set of reporting
regions specifically for the purpose of the Bureau’s Australian Water Resources Assessment
and are referred to as the 2010 and 2012 Assessment Reporting Regions.""" ;
  dc:source "Page 44 in the Australian Hydrological Geospatial Fabric (Geofabric) v3.0 Product Guide"@en ;
  rdfs:comment """The Geofabric's Hydrology Reporting Region product's AWRA Drainage Division object.

Drainage Division is defined for the purpose of providing a stable set of reporting regions specifically for the purpose of the Bureau’s Australian Water Resources Assessment (AWRA) and are referred to as the 2010 and 2012 Assessment Reporting Regions"""@en ;
  rdfs:label "Drainage Division" ;
  rdfs:subClassOf :ReportingRegion ;
  rdfs:subClassOf geo:Feature ;
  rdfs:subClassOf hyf:HY_CatchmentAggregate ;
.
:ReportingRegion
  a owl:Class ;
  dc:description """Geofabric Hydrology Reporting Regions are derived from aggregations of contracted
catchments from Geofabric Hydrology Reporting Catchments. This product contains two
candidate reporting regions, namely AWRA Drainage Division for national scale reporting
purposes and River Region for regional scale reporting purposes. More reporting regions may
be added in future releases based on user requirements.

The AWRA Drainage Division is defined for the purpose of providing a stable set of reporting
regions specifically for the purpose of the Bureau’s Australian Water Resources Assessment
and are referred to as the 2010 and 2012 Assessment Reporting Regions.

The River Regions were based on a specification developed by Bureau hydrologists involved in
water resources assessment in consultation with the Geofabric team and scientists from
CSIRO and ANU. These boundaries were developed for use in regional scale reporting and
hydrological modelling. The River Region boundaries were not used in the Australian Water
Resources Assessment 2010 and 2012 but may be considered in the future as the resolution
of reporting increases.

Though the Geofabric Hydrology Reporting Regions have been developed for the purposes of
the Australian Water Resources Assessment, it is envisaged that these units can be used more
generally as a standard for hydrological reporting at the national and regional scale, and thus
replace the Australia River Basins 1997 (http://www.ga.gov.au/metadatagateway/metadata/record/gcat_42343).
Table 31 shows the Geofabric Hydrology Reporting Regions feature class terminology and
feature subtypes. """ ;
  dc:source "Section 5.5 Page 44 in the Australian Hydrological Geospatial Fabric (Geofabric) v3.0 Product Guide"@en ;
  rdfs:label "Geofabric Hydrology reporting region" ;
  rdfs:subClassOf geo:Feature ;
  rdfs:subClassOf hyf:HY_CatchmentAggregate ;
.
:RiverRegion
  a owl:Class ;
  dc:description """The River Regions were based on a specification developed by Bureau hydrologists involved in
water resources assessment in consultation with the Geofabric team and scientists from
CSIRO and ANU. These boundaries were developed for use in regional scale reporting and
hydrological modelling. The River Region boundaries were not used in the Australian Water
Resources Assessment 2010 and 2012 but may be considered in the future as the resolution
of reporting increases.""" ;
  rdfs:comment """The Geofabric's Hydrology Reporting Region product's River Region object.

Reporting Regions are derived from aggregations of Contracted Catchments for regional scale reporting purposes.

A River Regions is always within one and only one Drainage Division."""@en ;
  rdfs:label "River Region" ;
  rdfs:subClassOf :ReportingRegion ;
  rdfs:subClassOf geo:Feature ;
  rdfs:subClassOf hyf:HY_CatchmentAggregate ;
  rdfs:subClassOf [
      a owl:Restriction ;
      owl:onClass :DrainageDivision ;
      owl:onProperty geo:sfWithin ;
      owl:qualifiedCardinality "1"^^xsd:nonNegativeInteger ;
    ] ;
.
dc:source
  a owl:AnnotationProperty ;
.
geo:Feature
  a owl:Class ;
.
sdo:identifier
  a owl:AnnotationProperty ;
.
sdo:name
  a owl:AnnotationProperty ;
.
hyf:HY_Catchment
  a owl:Class ;
  rdfs:comment "The HY Features Ontology's generic class for a catchment"@en ;
  rdfs:label "Catchment" ;
.
hyf:HY_CatchmentAggregate
  a owl:Class ;
  rdfs:comment "The HY Features Ontology's generic class for an aggregation of catchments"@en ;
  rdfs:label "Catchment Aggregate" ;
.
[
  sdo:identifier <http://catalogue.linked.data.gov.au/org/csiro> ;
  sdo:name "CSIRO" ;
].
[
  sdo:identifier <http://catalogue.linked.data.gov.au/org/csiro> ;
  sdo:name "CSIRO" ;
].
[
  sdo:identifier <http://catalogue.linked.data.gov.au/org/csiro> ;
  sdo:name "CSIRO" ;
].
[
  sdo:identifier <http://catalogue.linked.data.gov.au/org/csiro> ;
  sdo:name "CSIRO" ;
].
[
  sdo:identifier <http://orcid.org/0000-0002-8742-7730> ;
  sdo:name "Nicholas J. Car" ;
].
[
  sdo:identifier <http://orcid.org/0000-0002-8742-7730> ;
  sdo:name "Nicholas J. Car" ;
].
[
  sdo:identifier <http://orcid.org/0000-0002-8742-7730> ;
  sdo:name "Nicholas J. Car" ;
].
[
  sdo:identifier <http://orcid.org/0000-0002-8742-7730> ;
  sdo:name "Nicholas J. Car" ;
].
